WIP: JS.dfy: exploring Promises etc.

packages/zoe/spec/JS.dfy
@@ -1,19 +1,119 @@
+include "outcome.dfy"
 
-  module JS {
-    datatype Primitive = Undefined | Boolean(b: bool) | Number(x: int) |
-                         String(s: string) | Symbol(sym: string) | Bigint(i: int)
-    datatype Value = P(p: Primitive) | Object(o: object)
-    function typeof(v: Value): string {
-      match v {
-        case P(p) => match p {
-          case Undefined() => "undefined"
-          case Boolean(_) => "boolean"
-          case Number(_) => "number"
-          case String(_) => "string"
-          case Symbol(_) => "symbol"
-          case Bigint(_) => "bigint"
-        }
-        case Object(_) => "object"
+module {:options "--function-syntax:4"} JS {
+  import opened Outcome
+
+  function exp(b: nat, e: nat): nat
+    requires b > 0
+    ensures exp(b, e) >= 1
+  { if e == 0 then 1 else b * exp(b, e - 1) }
+  const MAX_SAFE_INT := exp(10, 53)
+  function Abs(x: int): nat { if x < 0 then -x else x }
+  type SafeInt = x: int | Abs(x) < MAX_SAFE_INT witness 1
+
+  // Rather than deal with floats, we stick to SafeInt
+  // is String colliding with something?
+  datatype Primitive = Undefined | Boolean(b: bool) | Number(x: SafeInt) |
+                       Str(s: string) | Symbol(sym: string) | Bigint(i: int)
+  datatype Value = Prim(p: Primitive) | Obj(o: object)
+  function undefined(): Value { Prim(Undefined) }
+  function strVal(s: string): Value { Prim(Str(s)) }
+  function okStr(s: string): Outcome<Value> { Success(Prim(Str(s))) }
+
+  function typeof(v: Value): string {
+    match v {
+      case Prim(p) => match p {
+        case Undefined() => "undefined"
+        case Boolean(_) => "boolean"
+        case Number(_) => "number"
+        case Str(_) => "string"
+        case Symbol(_) => "symbol"
+        case Bigint(_) => "bigint"
+      }
+      case Obj(x) => if x is Function then "function" else "object"
+    }
+  }
+
+  // :termination false means open to extension in other modules?
+  trait {:termination false} JsObj {
+    method Get(property: string) returns (out: Outcome<Value>)
+    method Call(args: seq<Value>) returns (out: Outcome<Value>)
+    // static method Construct(args: seq<Value>) returns (out: Outcome<Value>)
+    static  method fail(n: string, m: string) returns (out: Outcome<Value>) {
+      var err := new Error(n, m);
+      out := Failure(err);
+    }
+    static  method typeError(m: string) returns (out: Outcome<Value>) {
+      out := fail("TypeError", m);
+    }
+  }
+
+  trait NoProperties extends JsObj {
+    method Get(property: string) returns (out: Outcome<Value>) {
+      return Success(undefined());
+    }
+  }
+
+  class Error extends JsObj {
+    const name: string
+    const message: string
+    constructor(n: string, m: string)
+      ensures name == n && message == m
+    {
+      name, message := n, m;
+    }
+
+    method Get(property: string) returns (out: Outcome<Value>) {
+      match property {
+        case "message" => return okStr(message);
+        case _ => return Success(undefined());
+      }
+    }
+
+    method Call(args: seq<Value>) returns (out: Outcome<Value>) {
+      out := typeError("not a function");
+    }
+  }
+
+  trait Function extends JsObj {
+    function check(specimen: Value): bool {
+      match specimen {
+        case Obj(o) => o is Function
+        case _ => false
       }
     }
   }
+
+  datatype State = Pending | Fulfilled | Rejected
+  class Promise extends JsObj {
+    const executor: Function
+    var state: State
+    constructor(executor_: Function)
+      ensures state == Pending
+    {
+      state, executor := Pending, executor_;
+    }
+    method Get(property: string) returns (out: Outcome<Value>) {
+      match property {
+        case "then" =>
+          out := fail("TODO", "@@@");
+        case _ => return Success(undefined());
+      }
+    }
+    method Call(args: seq<Value>) returns (out: Outcome<Value>) {
+      out := typeError("not a function");
+    }
+  }
+
+  class Resolver extends Function, NoProperties {
+    const next: Function
+    constructor(next_: Function) {
+      next := next_;
+    }
+    method Call(args: seq<Value>) returns (out: Outcome<Value>) {
+      var res := if |args| > 0 then args[0] else undefined();
+      var args : seq<Value> := [Obj(next)];
+      out := next.Call(args); // termination?!
+    }
+  }
+}
